low star examples

examples/low-star/ml/CBuffer.ml
@@ -1,0 +1,3 @@
+
+(* Change content for base ptr *)
+type buffer = { content: char array; start_idx:int; length:int}
