examples/low-star/ml/CSystem.ml
@@ -1,0 +1,122 @@
+open CBuffer
+
+type fd = Unix.file_descr
+type buffer = { content : bytes; start_idx : int; length : int;}
+
+external ocaml_writev: fd -> buffer array -> int -> int = "ocaml_writev"
+external ocaml_readv: fd -> buffer array -> int -> int = "ocaml_readv"
+
+let char_array_to_bytes a =
+  let b = Bytes.create (Array.length a) in
+  for i = 0 to Array.length a - 1 do
+    Bytes.set b i a.(i)
+  done;
+  b
+
+let bytes_to_char_array a b =
+  for i = 0 to Array.length a - 1 do
+    a.(i) <- Bytes.get b i
+  done
+
+let cbuffer_to_buffer (cbuff:CBuffer.buffer) =
+  let (buff:buffer) = { content = char_array_to_bytes cbuff.content;
+                        start_idx = cbuff.start_idx;
+                        length = cbuff.length; } in
+  buff
+
+type open_flag =
+  | READ_ONLY
+  | WRITE_ONLY
+  | READ_WRITE
+  | APPEND
+  | CREATE
+
+let map_flag f =
+  match f with
+  | READ_ONLY -> Unix.O_RDONLY
+  | WRITE_ONLY -> Unix.O_WRONLY
+  | READ_WRITE -> Unix.O_RDWR
+  | APPEND -> Unix.O_APPEND
+  | CREATE -> Unix.O_CREAT
+  | _ -> failwith "Unhandled flag"
+
+let read f (b:CBuffer.buffer) idx len =
+  let buff = char_array_to_bytes b.content in
+  let n = Unix.read f buff idx len in
+  print_string ("Content read : " ^ (Bytes.sub_string buff 0 n) ^ "\n");
+  bytes_to_char_array b.content buff;
+  n
+
+let write = Unix.write
+let openfile f l i = Unix.openfile f (List.map map_flag l) i
+let close = Unix.close
+
+let readv fd buffers =
+  let buffs = Array.of_list buffers in
+  let buff_len = Array.length buffs in
+  ocaml_readv fd buffs buff_len
+
+let writev fd (buffers:CBuffer.buffer list) =
+  let buffs = Array.of_list buffers in
+  for i = 0 to Array.length buffs - 1 do
+    print_string "Buffer content :\n";
+    for j = buffs.(i).start_idx to buffs.(i).start_idx + buffs.(i).length do
+      print_char buffs.(i).content.(j) ;
+    done;
+    print_string "\n";
+  done;
+  let buff_len = Array.length buffs in
+  let buffs = Array.map cbuffer_to_buffer buffs in
+  ocaml_writev fd buffs buff_len
+
+(*
+let get_inet_tcp_socket = (fun ( _ ) -> (Support.All.failwith "Not yet implemented:get_inet_tcp_socket"))
+
+let accept = (fun ( f ) -> (Support.All.failwith "Not yet implemented:accept"))
+
+let bind = (fun ( _ ) ( _ ) ( _ ) -> (Support.All.failwith "Not yet implemented:bind"))
+
+let listen = (fun ( _ ) ( _ ) -> (Support.All.failwith "Not yet implemented:listen"))
+
+
+let is_O_RDONLY = (fun ( _discr_ ) -> (match (_discr_) with
+| Support.System.O_RDONLY -> begin
+true
+end
+| _ -> begin
+false
+end))
+
+let is_O_WRONLY = (fun ( _discr_ ) -> (match (_discr_) with
+| Support.System.O_WRONLY -> begin
+true
+end
+| _ -> begin
+false
+end))
+
+let is_O_RDWR = (fun ( _discr_ ) -> (match (_discr_) with
+| Support.System.O_RDWR -> begin
+true
+end
+| _ -> begin
+false
+end))
+
+let is_O_APPEND = (fun ( _discr_ ) -> (match (_discr_) with
+| Support.System.O_APPEND -> begin
+true
+end
+| _ -> begin
+false
+end))
+
+let is_O_CREAT = (fun ( _discr_ ) -> (match (_discr_) with
+| Support.System.O_CREAT -> begin
+true
+end
+| _ -> begin
+false
+end))
+
+*)
