examples/low-star/ml/cfun.c
@@ -1,0 +1,78 @@
+#include <stdlib.h>
+#include <stdio.h>
+#include <sys/uio.h>
+#include <caml/mlvalues.h>
+#include <caml/alloc.h>
+#include <caml/memory.h>
+
+typedef struct iovec buffer;
+
+// This function takes an array of OCaml bytes as argument
+CAMLprim value
+ocaml_writev(value f, value buffers, value nb_buffers)
+{
+  CAMLparam3( f, buffers, nb_buffers);
+  buffer *iov;
+  int i, n, filedes, iovcnt;
+  iov = (buffer *)malloc(sizeof(buffer) * iovcnt);
+
+  filedes = Int_val(f);
+  iovcnt = Int_val(nb_buffers);
+
+  for (i = 0; i < iovcnt; i++) {
+    iov[i].iov_base = String_val(Field(Field(buffers, i), 0))
+                      + Int_val(Field(Field(buffers, i), 1));
+    iov[i].iov_len = Int_val(Field(Field(buffers, i), 2));
+  }
+
+  n = (int)writev(filedes, iov, iovcnt);
+
+  return Val_int(n);
+}
+
+// This function takes an array of OCaml char array as argument
+/*
+CAMLprim value
+ocaml_writev2(value f, value buffers, value nb_buffers)
+{
+  CAMLparam3( f, buffers, nb_buffers);
+  buffer *iov;
+  int i, n, filedes, iovcnt;
+  iov = (buffer *)malloc(sizeof(buffer) * iovcnt);
+
+  filedes = Int_val(f);
+  iovcnt = Int_val(nb_buffers);
+
+  for (i = 0; i < iovcnt; i++) {
+    iov[i].iov_base = (Field(Field(buffers, i), 0))
+                      + Int_val(Field(Field(buffers, i), 1));
+    iov[i].iov_len = Int_val(Field(Field(buffers, i), 2));
+  }
+
+  n = (int)writev(filedes, iov, iovcnt);
+
+  return Val_int(n);
+}
+*/
+
+CAMLprim value
+ocaml_readv(value f, value buffers, value nb_buffers)
+{
+  CAMLparam3( f, buffers, nb_buffers);
+  buffer *iov;
+  int i, n, filedes, iovcnt;
+  iov = (buffer *)malloc(sizeof(buffer) * iovcnt);
+
+  filedes = Int_val(f);
+  iovcnt = Int_val(nb_buffers);
+
+  for (i = 0; i < iovcnt; i++) {
+    iov[i].iov_base = String_val(Field(Field(buffers, i), 0))
+                      + Int_val(Field(Field(buffers, i), 1));
+    iov[i].iov_len = Int_val(Field(Field(buffers, i), 2));
+  }
+
+  n = (int)readv(filedes, iov, iovcnt);
+
+  return Val_int(n);
+}
