examples/low-star/system.fst
@@ -1,10 +1,10 @@
 (*--build-config
-    options:--admit_fsi Set --admit_fsi Seq  --verify_module System --z3timeout 100;
+    options:--admit_fsi Set --admit_fsi Seq --verify_module System --z3timeout 10;
     variables:LIB=../../lib PLATFORM=../../contrib/Platform/fst SST=../low-level;
-  other-files:$LIB/classical.fst $LIB/ext.fst $LIB/set.fsi $LIB/seq.fsi $LIB/heap.fst $LIB/st.fst $LIB/all.fst $LIB/seqproperties.fst $LIB/list.fst $LIB/listTot.fst $SST/stack.fst $SST/listset.fst $LIB/ghost.fst $SST/located.fst $SST/lref.fst $SST/stackAndHeap.fst $SST/sst.fst $SST/sstCombinators.fst $SST/array.fsi $SST/array.fst buffer.fst
+  other-files:$LIB/classical.fst $LIB/ext.fst $LIB/set.fsi $LIB/seq.fsi $LIB/heap.fst $LIB/st.fst $LIB/all.fst $LIB/seqproperties.fst $LIB/list.fst $LIB/listTot.fst $LIB/listproperties.fst $SST/stack.fst $SST/listset.fst $LIB/ghost.fst $SST/located.fst $SST/lref.fst $SST/stackAndHeap.fst $SST/sst.fst $SST/sstCombinators.fst $SST/array.fsi $SST/array.fst buffer.fst
   --*)
 
-module System
+module CSystem
 
 open Set
 open Heap
@@ -16,18 +16,23 @@ open Located
 open SSTArray
 open Ghost
 
-open Buffer
+open CBuffer
 
 (* File descriptor : id * index *)
-type fd = nat * lref nat (* = ref nat * (idx:nat -> len:nat -> Tot byte) *)
+(* The file descriptor is currently represented as an int identifier
+   and a reference to an integer representing the current index the file is
+   at *)
+(* TODO : fix the representation & map it with whatever is returned by
+    the openfile function *)
+type fd = nat * lref nat
 
 (* Input stream to be read from a file descriptor *)
-assume val readStreamT : 
-  f:fd -> m:smem{liveRef (snd f) m} -> n:nat -> 
+assume val readStreamT :
+  f:fd -> m:smem{liveRef (snd f) m} -> n:nat ->
   Tot (s:(option (Seq.seq byte)){ is_Some s ==> Seq.length (Some.v s) <= n })
 
-assume val readStream : 
-  f:fd -> n:nat -> 
+assume val readStream :
+  f:fd -> n:nat ->
   PureMem (option (Seq.seq byte))
     (requires (fun m ->
     (liveRef (snd f) m)
@@ -36,44 +41,45 @@ assume val readStream :
       (liveRef (snd f) m)
       /\ (s = readStreamT f m n)
      ))
-       	   
+
 (* System read function *)
 assume val read :
   f:fd ->
-  b:buffer -> 
-  count:nat{ count <= b.length } -> 
+  b:buffer ->
+  off:nat{ off >= b.start_idx} ->
+  count:nat{ count <= reveal b.length } ->
   Mem nat
-    (requires (fun m -> 
+    (requires (fun m ->
       (liveBuffer m b)
       /\ (liveRef (snd f) m)
      ))
     (ensures (fun m0 n m1 ->
       (liveBuffer m0 b) /\ (liveBuffer m1 b)
       /\ (liveRef (snd f) m0)
-      /\ (is_Some (readStreamT f m0 count) ==> 
+      /\ (is_Some (readStreamT f m0 count) ==>
 	    (n = Seq.length (Some.v (readStreamT f m0 count))
-	    /\ (EqSub (sel m1 b.content) b.start_idx (Some.v (readStreamT f m0 count)) 0 n)))
-      /\ (EqSubInv (sel m0 b.content) (sel m1 b.content) b.start_idx count)
+	    /\ (EqSub (sel m1 b.content) off (Some.v (readStreamT f m0 count)) 0 n)))
+      /\ (EqSubInv (sel m0 b.content) (sel m1 b.content) off count)
      ))
     (eunion (eonly b.content) (only (snd f)))
 
 (* Output stream to write to a file descriptor *)
-assume val writeStreamT : 
-  f:fd -> m:smem{liveRef (snd f) m} -> b:buffer{liveBuffer m b} -> 
-  Tot (n:nat{n <= b.length})
+assume val writeStreamT :
+  f:fd -> m:smem{liveRef (snd f) m} -> b:buffer{liveBuffer m b} ->
+  Tot (n:nat{n <= reveal b.length})
 
 assume val write :
   f:fd ->
-  b:buffer -> 
+  b:buffer ->
   Mem nat
-    (requires (fun m -> 
+    (requires (fun m ->
       (liveBuffer m b)
       /\ (liveRef (snd f) m)
      ))
     (ensures (fun m0 n m1 ->
       (liveBuffer m0 b) /\ (liveBuffer m1 b)
       /\ (liveRef (snd f) m0) /\ (liveRef (snd f) m1)
-      /\ (n <= b.length /\ n >= 0) (* Issue : does not get it from the returned type *)
+      /\ (n <= reveal b.length /\ n >= 0) (* Issue : does not get it from the returned type *)
       /\ (is_Some (readStreamT f m1 n) /\ Seq.length (Some.v (readStreamT f m1 n)) = n)
       /\ (EqSub (Some.v (readStreamT f m1 n)) 0 (sel m0 b.content) b.start_idx n)
      ))
@@ -87,38 +93,41 @@ let rec setOfList l =
 
 val refSetFromBufferList : #a:Type -> list buffer -> Tot modset
 let rec refSetFromBufferList l =
-  match l with 
+  match l with
   | [] -> hide empty
   | hd::tl -> eunion (eonly hd.content) (refSetFromBufferList tl)
 
 (* Specification of the system call readv *)
-assume val readv : 
-    f:fd -> 
-    l:list buffer -> 
+(* TODO : write in terms of specs of read *)
+assume val readv :
+    f:fd ->
+    l:list buffer ->
     Mem nat
-      (requires (fun m -> 
-	(AllDistinct m l)
-	/\ (liveRef (snd f) m)
+      (requires (fun m ->
+	           (AllDistinct m l)
+	            /\ (liveRef (snd f) m)
        ))
       (ensures (fun m0 n m1 ->
-	(AllDistinct m0 l) /\ (AllDistinct m1 l)
-	/\ (liveRef (snd f) m0)
-	/\ (forall (b:buffer{List.mem b l}). glength b.content m0 = glength b.content m1)
-	/\ (bufferListLength m0 l = bufferListLength m1 l)
-	/\ (is_Some (readStreamT f m0 (bufferListLength m0 l)) ==> 
-	      (n = Seq.length (Some.v (readStreamT f m0 (bufferListLength m0 l)))
-	      /\ (Seq.Eq (Seq.slice (bufferListContent m1 l) 0 n) (Some.v (readStreamT f m0 (bufferListLength m0 l))))))
-	/\ (forall (b:buffer{List.mem b l}) (i:nat{i < glength b.content m0}).
-	      inBufferComplement m0 b i l ==> Seq.index (sel m0 b.content) i = Seq.index (sel m1 b.content) i)
+	         (AllDistinct m0 l) /\ (AllDistinct m1 l)
+	          /\ (liveRef (snd f) m0)
+	           /\ (forall (b:buffer{List.mem b l}). glength b.content m0 = glength b.content m1)
+	            /\ (bufferListLength m0 l = bufferListLength m1 l)
+	             /\ (is_Some (readStreamT f m0 (bufferListLength m0 l)) ==>
+	              (n = Seq.length (Some.v (readStreamT f m0 (bufferListLength m0 l)))
+	               /\ (Seq.Eq (Seq.slice (bufferListContent m1 l) 0 n) (Some.v (readStreamT f m0 (bufferListLength m0 l))))))
+	                /\ (forall (b:buffer{List.mem b l}) (i:nat{i < glength b.content m0}).
+	                 inBufferComplement m0 b i l ==> Seq.index (sel m0 b.content) i = Seq.index (sel m1 b.content) i)
        ))
       (eunion (refSetFromBufferList l) (only (snd f)))
 
 (* Specification of the system call writev *)
+(* TODO : fix wrong speficification about the input being disjoints, it should
+   not be the case for writev at least. *)
 assume val writev:
     f:fd ->
     l:list buffer ->
     Mem nat
-      (requires (fun m -> 
+      (requires (fun m ->
 	(AllDistinct m l)
 	/\ (liveRef (snd f) m)
        ))
@@ -128,5 +137,48 @@ assume val writev:
 	/\ (n <= bufferListLength m0 l /\ n >= 0)
 	/\ (is_Some (readStreamT f m1 n) /\ Seq.length (Some.v (readStreamT f m1 n)) = n)
 	/\ (Some.v (readStreamT f m1 n) = Seq.slice (bufferListContent m0 l) 0 n)
-       ))    
+       ))
       (only (snd f))
+
+(* Returns a inet datagram socket e.g. socket(AF_INET, SOCK_DGRAM,0) *)
+assume val get_inet_tcp_socket: unit ->
+  PureMem fd
+    (requires (fun m -> True))
+    (ensures (fun m v -> True))
+
+(* Accept connections on a socket, returns a socket connected to the client and
+its address *)
+assume val accept:
+  f:fd ->
+  PureMem (fd * string)
+    (requires (fun m -> True))
+    (ensures (fun m v -> True))
+
+assume val bind: fd -> string -> int ->
+  PureMem unit
+    (requires (fun m -> True))
+    (ensures (fun m v -> True))
+
+assume val listen:
+  fd -> int ->
+  PureMem unit
+    (requires (fun m -> True))
+    (ensures (fun m v -> True))
+
+type file_perm = int
+
+type open_flag =
+  | READ_ONLY
+  | WRITE_ONLY
+  | READ_WRITE
+  | APPEND
+  | CREATE
+
+(* TODO : create a ghost "content" associated to the filedescriptor (and
+   the memory state ?) *)
+assume val openfile:
+  string -> list open_flag -> file_perm ->
+  PureMem fd
+    (requires (fun m -> True))
+    (ensures (fun m f -> liveRef (snd f) m))
+assume val close: fd -> Tot unit
